High-level vale mem semantics (without store)

src/test/interop/Low_Sem.fst
@@ -1,25 +1,133 @@
 module Low_Sem
 
-module M = Memory
-open Machine
+module List = FStar.List.Tot.Base
+module M = Vale_Sem
+module B = FStar.Buffer
+module HS = FStar.HyperStack
+open Machine_int
+open Interop64
 
-type mem = M.heap
+type heap = M.heap
 
-noeq type state = {
-  ok:bool;
-  regs : reg -> nat64;
-  mem: mem;
+let buffer64 = B.buffer UInt64.t
+let buffer_addr (b:buffer64) (addrs:addr_map) =
+  addrs.[(B.as_addr b, B.idx b, B.length b)]
+  
+let buffer_read (b:buffer64) (i:nat{i < B.length b}) (mem:HS.mem) : GTot nat64 =
+  let contents = B.as_seq mem b in
+  UInt64.v (Seq.index contents i)
+
+let buffer_write (b:buffer64) (i:nat{i < B.length b}) (v:nat64) (mem:HS.mem) : GTot HS.mem =
+  admit()
+
+noeq type low_state_p = {
+  s:M.state;
+  addrs:addr_map;
+  ptrs: list buffer64;
+  mem: HS.mem;
 }
 
-let eval_reg (r:reg) (s:state) : nat64 = s.regs r
+let valid_state s =
+  list_disjoint_or_eq s.ptrs /\
+  s.s.M.mem == down_mem64 s.mem s.addrs s.ptrs
 
-let eval_maddr (m:maddr) (s:state) : int =
-  match m with
-  | MConst n -> n
-  | MReg r offset -> (eval_reg r s) + offset
+type low_state = (s:low_state_p{valid_state s})
 
-val valid_mem: ptr:int -> h:mem -> bool
-assume val load_mem: ptr:int -> h:mem -> nat64
-assume val store_mem: ptr:int -> v:nat64 -> h:mem -> mem
+val valid_mem: ptr:int 
+  -> s:low_state
+  -> GTot bool
+val load_mem: ptr:int 
+  -> s:low_state
+  -> GTot nat64
+val store_mem: ptr:int 
+  -> v:nat64 
+  -> s:low_state
+  -> GTot low_state
 
-let valid_mem ptr h = if ptr < 0 then false else not (M.addr_unused_in ptr h)
+val addr_in_ptr: (addr:int) -> (ptr:buffer64) -> (addrs:addr_map) ->
+  GTot (b:bool{ not b <==> (forall i. 0 <= i /\ i < B.length ptr ==> 
+    addr <> (buffer_addr ptr addrs) + 8 `op_Multiply` i)})
+  
+// Checks if address addr corresponds to one of the elements of buffer ptr
+let addr_in_ptr (addr:int) (ptr:buffer64) (addrs:addr_map) =
+  let n = B.length ptr in
+  let base = buffer_addr ptr addrs in
+  let rec aux (i:nat) : Tot (b:bool{not b <==> (forall j. i <= j /\ j < n ==> 
+    addr <> base + 8 `op_Multiply` j)}) 
+    (decreases %[n-i]) =
+    if i >= n then false
+    else if addr = base + 8 `op_Multiply` i then true
+    else aux (i+1)
+  in aux 0
+
+
+let rec valid_mem_aux addr ps (addrs:addr_map) : GTot (b:bool{
+  (not b) <==> (forall (x:buffer64). (List.memP x ps ==> not (addr_in_ptr addr x addrs) ))}) 
+  = match ps with
+    | [] -> false
+    | a::q -> if (addr_in_ptr addr a addrs) then true else valid_mem_aux addr q addrs
+
+let valid_mem addr s =
+  // Iterate over the list of buffers existing in this state
+  valid_mem_aux addr s.ptrs s.addrs
+
+
+let load_mem ptr s = M.get_heap_value ptr s.s
+
+let store_mem ptr v s =
+  let s' = M.update_mem ptr v s.s in
+  admit()
+
+let rec valid_mem_aux_lemma addr ps addrs (x:buffer64) : Lemma (
+   List.memP x ps /\ addr_in_ptr addr x addrs ==>
+   valid_mem_aux addr ps addrs
+   ) =
+   match ps with
+     | [] -> ()
+     | a::q -> valid_mem_aux_lemma addr q addrs x
+
+val lemma_valid_mem: b:buffer64
+  -> i:nat 
+  -> s:low_state
+  -> Lemma (requires i < B.length b /\ List.memP b s.ptrs)
+     (ensures valid_mem 
+       (buffer_addr b s.addrs + 8 `op_Multiply` i)
+       s)
+
+let lemma_valid_mem b i s =
+  let base = buffer_addr b s.addrs in
+  let addr = base + 8 `op_Multiply` i in
+  valid_mem_aux_lemma addr s.ptrs s.addrs b
+
+val lemma_load_mem: b:buffer64
+  -> i:nat
+  -> s:low_state
+  -> Lemma (requires i < B.length b /\ List.memP b s.ptrs)
+     (ensures load_mem (buffer_addr b s.addrs + 8 `op_Multiply` i) s == buffer_read b i s.mem)
+
+let lemma_load_mem b i s = ()
+
+val lemma_store_mem: b:buffer64 
+  -> i:nat 
+  -> v:nat64
+  -> s:low_state
+  -> Lemma (requires i < B.length b /\ List.memP b s.ptrs)
+     (ensures (store_mem (buffer_addr b s.addrs + 8 `op_Multiply` i) v s).mem == buffer_write b i v s.mem)
+
+val lemma_store_load_mem: i:int 
+  -> v:nat64
+  -> s:low_state
+  -> Lemma (load_mem i (store_mem i v s) == v)
+
+val lemma_frame_store_mem: i:int 
+  -> v:nat64
+  -> s:low_state
+  -> Lemma (let s' = store_mem i v s in
+     forall i'. i' <> i /\ valid_mem i s /\ valid_mem i' s ==> 
+       load_mem i' s = load_mem i' s')
+
+val lemma_valid_store_mem: i:int 
+  -> v:nat64
+  -> s:low_state
+  -> Lemma (let s' = store_mem i v s in
+     forall j. valid_mem j s <==> valid_mem j s')
